Security Length Lemma

theory/System/PathORAMSecurity.v
@@ -12,6 +12,7 @@ Require Import POram.Utils.Lists.
 Require Import POram.Utils.Vectors.
 Require Import POram.Utils.Tree.
 Require Import POram.Utils.Rationals.
+Require Import POram.Utils.StateT.
 Require Import POram.Utils.Distributions.
 Require Import POram.System.PathORAMDef.
 Require Import POram.System.PathORAMFunCorrect.
@@ -87,6 +88,7 @@ Definition monad_map {A B M} `{Monad M} (f : A -> B) (a : M A) : M B :=
   x <- a ;;
   mreturn (f x).
 
+
 (* Definition acc_list_1 {C : Config} (arg_list : list (block_id * operation)) (s : state) : *)
 (*   list (dist path). *)
 (*   pose (List.map (fun '(bid, op) => access bid op) arg_list). *)
@@ -99,23 +101,63 @@ Definition monad_map {A B M} `{Monad M} (f : A -> B) (a : M A) : M B :=
 (* Defined. *)
 
 Definition acc_dist_list {C : Config}
-  (arg_list : list (block_id * operation)) (s : state) : dist (list bool):=
+  (arg_list : list (block_id * operation)) : Poram (list path) :=
   let l := List.map (fun '(bid, op) => access bid op) arg_list in
   let p := sequence l in
-  let p_l := monad_map (List.map fst) p in
-  monad_map (@List.concat bool) (monad_map fst (p_l s)).
+  monad_map (List.map fst) p.
+
+Definition get_dist_list_bool {C : Config}
+  (arg_list : list (block_id * operation))(s : state) : dist (list bool) :=
+  monad_map (@List.concat bool) (monad_map fst ((acc_dist_list arg_list) s)).
 
 Lemma plift_monad_map : forall {X Y} (f : X -> Y) (d : dist X) (P : Y -> Prop), 
     plift (fun x => P (f x)) d -> 
     plift P (monad_map f d).
+Proof.
+  intros.
+  eapply plift_bind.
+  - exact H.
+  - intros. 
+    eapply plift_ret.
+    apply H0; auto.
+Qed.
+
+Lemma state_plift_monad_map :
+  forall {X Y} (Pre Post: state -> Prop) (P : Y -> Prop)
+    (f : X -> Y) (m : Poram X),
+    state_plift Pre Post (fun x => P (f x)) m ->
+    state_plift Pre Post P (monad_map f m).
+Proof.
+  intros.
+  eapply state_plift_bind.
+  - exact H.
+  - intros. 
+    eapply state_plift_ret.
+    apply H0; auto.
+Qed.
+
+Lemma acc_dist_list_length :
+  forall {C : Config} (arg_list : list (block_id * operation)),
+    state_plift (fun _ => True) (fun _ => True)
+      (fun l => List.length l = List.length arg_list /\ (Forall (fun l' => List.length l' = LOP) l)) (acc_dist_list arg_list).
 Admitted.
+
 
 Theorem arg_list_len_rel :
-  forall {C : Config} (arg_list : list (block_id * operation)) (s : state),
+  forall {C : Config} (arg_list : list (block_id * operation))(s : state),
     plift (fun l => List.length l = List.length arg_list * LOP)%nat
-      (acc_dist_list arg_list s).
-Admitted.
-
+      (get_dist_list_bool arg_list s).
+Proof.
+  intros.
+  do 2 apply plift_monad_map.
+  pose proof (acc_dist_list_length arg_list s I).
+  eapply dist_has_weakening; [ | exact H].
+  intros.
+  simpl in H0. destruct x. destruct H0. simpl.
+  destruct H0.
+Admitted. 
+  
+  
 (* TODO: fix the probability *)
 Definition uniform (n : nat) (d : dist (list bool)) :=
   forall l, (List.length l = n)%nat ->
@@ -126,7 +168,7 @@ Definition uniform (n : nat) (d : dist (list bool)) :=
 Theorem access_dist_preservation :
   forall {C : Config} (arg_list : list (block_id * operation)) (s : state),
     uniform ((List.length arg_list) * LOP)
-      (acc_dist_list arg_list s).
+      (get_dist_list_bool arg_list s).
 Admitted.
 
 
